work on module-ifying

concurrency/framework/PCM.s.dfy
@@ -9,11 +9,6 @@ abstract module PCM {
 
   type M(!new)
 
-  type {:extern} Token(!new) {
-    function {:extern} loc() : Loc
-    function {:extern} get() : M
-  }
-
   // Partial Commutative Monoid (PCM) axioms
 
   function unit() : M
@@ -55,67 +50,76 @@ abstract module PCM {
   requires dot_defined(a, c)
   ensures dot_defined(b, c)
   ensures transition(dot(a, c), dot(b, c))
+}
+
+module Tokens(pcm: PCM) {
+  import opened GhostLoc
 
   /*
    * Actions
    */
 
+  type {:extern} Token(!new) {
+    function {:extern} loc() : Loc
+    function {:extern} get() : pcm.M
+  }
+
   function method {:extern} transition_update(
       gshared s: Token,
       glinear b: Token,
-      ghost expected_out: M)
+      ghost expected_out: pcm.M)
     : (glinear c: Token)
   requires s.loc() == b.loc()
-  requires dot_defined(s.get(), b.get()) ==>
-    dot_defined(s.get(), expected_out)
-      && transition(
-        dot(s.get(), b.get()),
-        dot(s.get(), expected_out))
+  requires pcm.dot_defined(s.get(), b.get()) ==>
+    pcm.dot_defined(s.get(), expected_out)
+      && pcm.transition(
+        pcm.dot(s.get(), b.get()),
+        pcm.dot(s.get(), expected_out))
   ensures c.get() == expected_out
   ensures c.loc() == s.loc()
 
   function method {:extern} get_unit(ghost loc: Loc) : (glinear u: Token)
-  ensures u.get() == unit() && u.loc() == loc
+  ensures u.get() == pcm.unit() && u.loc() == loc
 
   glinear method {:extern} dispose(glinear u: Token)
 
   function method {:extern} get_unit_shared(ghost loc: Loc) : (gshared u: Token)
-  ensures u.get() == unit() && u.loc() == loc
+  ensures u.get() == pcm.unit() && u.loc() == loc
 
   // This MUST be 'method', as it wouldn't be safe to call this and
   // obtain the postconditions from only ghost 'a' and 'b'.
   glinear method {:extern} join(glinear a: Token, glinear b: Token)
   returns (glinear sum: Token)
   requires a.loc() == b.loc()
-  ensures dot_defined(a.get(), b.get()) // yes, this is an 'ensures'
-  ensures sum.get() == dot(a.get(), b.get())
+  ensures pcm.dot_defined(a.get(), b.get()) // yes, this is an 'ensures'
+  ensures sum.get() == pcm.dot(a.get(), b.get())
   ensures sum.loc() == a.loc()
 
   // Same as above: must be 'method', not 'function method'
   glinear method {:extern} is_valid(gshared a: Token, glinear inout b: Token)
   requires a.loc() == old_b.loc()
   ensures b == old_b
-  ensures dot_defined(a.get(), b.get())
+  ensures pcm.dot_defined(a.get(), b.get())
 
   // The only reason this is a 'method' and not a 'function method'
   // is so it can easily have two return args.
-  glinear method {:extern} split(glinear sum: Token, ghost a: M, ghost b: M)
+  glinear method {:extern} split(glinear sum: Token, ghost a: pcm.M, ghost b: pcm.M)
   returns (glinear a': Token, glinear b': Token)
-  requires dot_defined(a, b)
-  requires sum.get() == dot(a, b)
+  requires pcm.dot_defined(a, b)
+  requires sum.get() == pcm.dot(a, b)
   ensures a'.get() == a && a'.loc() == sum.loc()
   ensures b'.get() == b && b'.loc() == sum.loc()
 
-  function method {:extern} join_shared(gshared s: Token, gshared t: Token, ghost expected_q: M)
+  function method {:extern} join_shared(gshared s: Token, gshared t: Token, ghost expected_q: pcm.M)
     : (gshared q: Token)
-  requires forall r :: le(s.get(), r) && le(t.get(), r) ==> le(expected_q, r)
+  requires forall r :: pcm.le(s.get(), r) && pcm.le(t.get(), r) ==> pcm.le(expected_q, r)
   requires s.loc() == t.loc()
   ensures q.get() == expected_q
   ensures q.loc() == s.loc()
 
-  function method {:extern} sub(gshared s: Token, ghost t: M)
+  function method {:extern} sub(gshared s: Token, ghost t: pcm.M)
    : (glinear t': Token)
-  requires le(t, s.get())
+  requires pcm.le(t, s.get())
   ensures t'.get() == t
   ensures t'.loc() == s.loc()
 }
