concurrency/framework/PCMExt.s.dfy
@@ -1,8 +1,6 @@
 include "PCM.s.dfy"
 
-abstract module PCMExt refines PCM {
-  import Base : PCM
-
+abstract module PCMExt(Base: PCM) refines PCM {
   type B = Base.M
   type F = M
 
@@ -22,12 +20,20 @@ abstract module PCMExt refines PCM {
   requires transition(f, f')
   ensures Base.reachable(b, b')
   ensures dot_defined(f', p) && rep(dot(f', p), b')
+}
+
+module PCMExtMethods(Base: PCM, Ext: PCMExt(Base)) {
+  type B = Base.M
+  type F = Ext.M
+
+  import BaseTokens = Tokens(Base)
+  import ExtTokens = Tokens(Ext)
 
   function method {:extern} ext_init(
-      glinear b: Base.Token,
+      glinear b: BaseTokens.Token,
       ghost f': F)
-   : (glinear f_out: Token)
-  requires rep(f', b.get())
+   : (glinear f_out: ExtTokens.Token)
+  requires Ext.rep(f', b.get())
   ensures f_out.loc().ExtLoc? && f_out.loc().base_loc == b.loc()
   ensures f_out.get() == f'
 
@@ -35,16 +41,16 @@ abstract module PCMExt refines PCM {
   // (Remember there is NO SOUND VERSION that accepts a `gshared b`)
 
   glinear method {:extern} ext_transfer(
-      glinear f: Token,
+      glinear f: ExtTokens.Token,
       ghost f': F,
-      glinear b: Base.Token,
+      glinear b: BaseTokens.Token,
       ghost b': B)
-  returns (glinear f_out: Token, glinear b_out: Base.Token)
+  returns (glinear f_out: ExtTokens.Token, glinear b_out: BaseTokens.Token)
   requires f.loc().ExtLoc? && f.loc().base_loc == b.loc()
-  requires forall p, q :: dot_defined(f.get(), p) && rep(dot(f.get(), p), q) && Base.dot_defined(q, b.get()) ==>
+  requires forall p, q :: Ext.dot_defined(f.get(), p) && Ext.rep(Ext.dot(f.get(), p), q) && Base.dot_defined(q, b.get()) ==>
     exists q' ::
-      dot_defined(f', p) &&
-      rep(dot(f', p), q') &&
+      Ext.dot_defined(f', p) &&
+      Ext.rep(Ext.dot(f', p), q') &&
       Base.dot_defined(q', b') &&
       Base.reachable(Base.dot(q, b.get()), Base.dot(q', b'))
   ensures f_out.loc() == f.loc()
@@ -52,25 +58,25 @@ abstract module PCMExt refines PCM {
   ensures f_out.get() == f'
   ensures b_out.get() == b'
 
-  function method {:extern} borrow_back(gshared f: Token, ghost b: B)
-    : (gshared b_out: Base.Token)
+  function method {:extern} borrow_back(gshared f: ExtTokens.Token, ghost b: B)
+    : (gshared b_out: BaseTokens.Token)
   requires f.loc().ExtLoc?
   requires forall p, b1 ::
-      dot_defined(f.get(), p) && rep(dot(f.get(), p), b1) ==> Base.le(b, b1)
+      Ext.dot_defined(f.get(), p) && Ext.rep(Ext.dot(f.get(), p), b1) ==> Base.le(b, b1)
   ensures b_out.get() == b
   ensures b_out.loc() == f.loc().base_loc
 
   glinear method {:extern} exists_whole(
-      gshared s: Token,
-      glinear inout f: Token,
-      glinear inout b: Base.Token)
+      gshared s: ExtTokens.Token,
+      glinear inout f: ExtTokens.Token,
+      glinear inout b: BaseTokens.Token)
   returns (ghost res: F, ghost b': Base.M)
   requires s.loc() == old_f.loc()
   requires s.loc().ExtLoc? && s.loc().base_loc == old_b.loc()
   ensures f == old_f
   ensures b == old_b
-  ensures dot_defined(s.get(), f.get())
-  ensures dot_defined(dot(s.get(), f.get()), res)
-  ensures rep(dot(dot(s.get(), f.get()), res), b')
+  ensures Ext.dot_defined(s.get(), f.get())
+  ensures Ext.dot_defined(Ext.dot(s.get(), f.get()), res)
+  ensures Ext.rep(Ext.dot(Ext.dot(s.get(), f.get()), res), b')
   ensures Base.dot_defined(b', b.get())
 }
